refactoring linked lists (part 1)

state/LinkedListIFC.fst
@@ -4,102 +4,24 @@ open FStar.Tactics
 open FStar.Tactics.Typeclasses
 open Monotonic.IFC.Heap
 open IFC.Heap.ST
+open FStar.Ghost
 
 open STLC
 open TargetLangIFC
 
-noeq type linkedList (a: Type0) : Type0 =
-    | Nil
-    | Cons of a * ref (linkedList a)
+module FSet = FStar.FiniteSet.Base
 
-instance target_lang_linkedList (t1:Type) {| c1:target_lang t1 |} : target_lang (linkedList t1) = {
-  shallowly_contained = (fun l h ->
+let head_tot (#a: Type0) (l: linkedList a{l =!= Nil}) (h: lheap) {| c: witnessable a |} : a =
+  let Cons(x, xsref) = l in
+ x
+
+let tail_tot (#a: Type0) (l: linkedList a) (h: lheap) {| c: witnessable a |} : linkedList a = 
     match l with
-    | Nil -> True
-    | Cons (x, xs) -> c1.shallowly_contained x h /\ is_mm xs = false /\ contains_pred xs h); 
-  shallowly_low = (fun l h ->
-    match l with
-    | Nil -> True
-    | Cons (x, xs) -> c1.shallowly_low x h /\ is_low_pred xs h);
-  shallowly_witness = (fun l ->
-    match l with 
-    | Nil -> (fun () -> ())
-    | Cons (x, xs) ->
-      let w = c1.shallowly_witness x in
-      gst_witness (contains_pred xs);
-      gst_witness (is_low_pred xs);
-      (fun () -> w ();
-       gst_recall (contains_pred xs);
-       gst_recall (is_low_pred xs))
-      )
-}
-
-// maybe change this to not use IST
-let head (a: Type0) (l:linkedList a) {| c1:target_lang a |} : IST (option a)
-  (requires (fun h -> shallowly_contained l h))
-    (ensures fun _ _ _ -> True) = 
-      match l with
-      | Nil -> None
-      | Cons (x, xsref) -> Some x
-
-let tail (a: Type0) (l: linkedList a) {| c1:target_lang a |} : IST (linkedList a)
-    (requires (fun h -> shallowly_contained l h))
-    (ensures fun _ _ _ -> True) = 
-      match l with
       | Nil -> Nil
-      | Cons (x, xsref) -> !xsref
+      | Cons (x, xsref) -> 
+        assume (satisfy l h contains_pred);
+        sel_tot h xsref
 
-let rec last (#a: Type0) (l:linkedList a) {| c1:target_lang a |} : IST (option a)
-  (requires (fun h -> shallowly_contained l h))
-  (ensures fun _ _ _ -> True) = 
-    let h0 = get() in
-    match l with 
-    | Nil -> None
-    | Cons (x, xsref) ->
-      let xs = !xsref in
-      match xs with
-      | Nil -> Some x
-      | Cons _ -> 
-        eliminate forall (a:Type) (c:target_lang a) (r':ref a). shallowly_contained r' h0 ==>
-          c.shallowly_contained (sel h0 r') h0 with (linkedList a) (solve) xsref;
-        last xs #c1
-
-let insert_front (a: Type0) (l: linkedList a) (v: a) {| c:target_lang a |}: ST (linkedList a)
-    (requires (fun _ -> True))
-    (ensures fun _ _ _ -> True) = 
-    let r: ref (linkedList a) = alloc l in 
-    Cons (v, r)
-
-// TODO: fix this
-// let rec append (a: Type0) (l: linkedList a) (v: a) {| c:target_lang a |}: IST (linkedList a)
-//     (requires (fun h -> shallowly_witnessed_contains l /\ shallowly_witnessed_is_low l))
-//     (ensures fun _ _ _ -> True) =
-//     let h0 = get() in
-//     match l with 
-//     | Nil -> 
-//       let r = alloc Nil in 
-//       Cons (v, r)
-//     | Cons (v, r) -> 
-//       let tl = !r in
-//         eliminate forall (a:Type) (c:target_lang a) (r':ref a). witnessed (is_low_pred r') ==>
-//         c.shallowly_witnessed_is_low (sel h0 r') with (linkedList a) (solve) r;
-//         append a tl v #c
-
-let rec length (a: Type0) (l: linkedList a) {| c:target_lang a |} : IST nat 
-       (requires (fun h -> shallowly_contained l h /\ shallowly_low l h))
-       (ensures fun _ _ _ -> True) =
-       let h0 = get() in
-        match l with 
-         | Nil -> 0
-         | Cons (x, xsref) -> 
-           let xs = !xsref in
-            eliminate forall (a:Type) (c:target_lang a) (r:ref a). shallowly_low r h0 ==>
-              c.shallowly_low (sel h0 r) h0 with (linkedList a) (solve) xsref;
-            eliminate forall (a:Type) (c:target_lang a) (r:ref a). shallowly_contained r h0 ==>
-              c.shallowly_contained (sel h0 r) h0 with (linkedList a) (solve) xsref;
-            1 + length a xs #c
-
-// cycles??
 let rec ll_eq (#a: Type0) (fuel: nat) (l1: linkedList a) (l2: linkedList a) (h: lheap) : Type0 =
   if fuel = 0 then True
   else
@@ -112,8 +34,109 @@ let rec ll_eq (#a: Type0) (fuel: nat) (l1: linkedList a) (l2: linkedList a) (h: 
       let ys = sel h ysref in  
       x == y /\ ll_eq (fuel - 1) xs ys h
 
-noeq
-type ll_constant_ind (#a: Type0) (h1 h2: lheap) : linkedList a -> Type0 =
+let head (#a: Type0) (l:linkedList a) {| c:witnessable a |} : IST (option a)
+  (requires fun h -> l =!= Nil)
+  (ensures fun h0 head h1 -> modifies_none h0 h1 /\ head == Some (head_tot l h1)) =
+      match l with
+      | Nil -> None
+      | Cons (x, xsref) -> Some x
+
+let tail (a: Type0) (l: linkedList a) {| c:witnessable a |} : IST (linkedList a)
+    (requires fun h -> satisfy l h contains_pred)
+    // try to use tail_tot in the postcondition
+    (ensures fun h0 xs h1 -> True) = 
+      match l with
+      | Nil -> Nil
+      | Cons (x, xsref) -> !xsref
+
+(* TODO: can we do this for l: linkedlist a? *)
+  // let rec last_elem (l: linkedList nat) {| c:witnessable nat |} : IST (option nat)
+  // (requires (fun h -> satisfy l h contains_pred))
+  // (ensures fun _ _ _ -> True) = 
+  //   let h0 = get() in
+  //   match l with 
+  //   | Nil -> None
+  //   | Cons (x, xsref) ->
+  //     let xs = !xsref in
+  //     match xs with
+  //     | Nil -> Some x
+  //     | Cons _ -> 
+  //       eliminate_inv_contains h0 (TLList TNat) xsref;
+  //       last_elem xs #c
+
+// let rec last_ref (#a: Type0) (l:linkedList a{l =!= Nil}) (h: lheap) : GTot (ref (linkedList a)) =
+//   let Cons (x, xsref) = l in
+//   assume (h `contains` xsref);
+//    let xs = sel h xsref in
+//    match xs with
+//     | Nil -> xsref
+//     | Cons _ -> last_ref #a xs h
+
+
+let insert_front (a: Type0) (l: linkedList a) (v: a) {| c:witnessable a |}: ST (linkedList a)
+    (requires (fun _ -> True))
+    (ensures fun _ _ _ -> True) = 
+    let r: ref (linkedList a) = alloc l in 
+    Cons (v, r)
+
+// TODO: fix this
+// let rec append (a: Type0) (l: linkedList a) (v: a) {| c:target_lang a |}: IST (linkedList a)
+//     (requires (fun h -> shallowly_contained l h /\ shallowly_low l h))
+//     (ensures fun _ _ _ -> True) =
+//     let h0 = get() in
+//     match l with
+//     | Nil -> 
+//       let r = alloc Nil in 
+//       Cons (v, r)
+//     | Cons (v, r) -> 
+//       let tl = !r in
+//         eliminate forall (a:Type) (c:target_lang a) (r':ref a). shallowly_low r' h0 ==>
+//         c.shallowly_low (sel h0 r') h0 with (linkedList a) (solve) r;
+//         append a tl v #c
+
+// let rec length_IST (a: Type0) (l: linkedList a) {| c:witnessable a |} : IST nat 
+//        (requires (fun h -> shallowly_contained_low l h))
+//        (ensures fun _ _ _ -> True) =
+//        let h0 = get() in
+//         match l with 
+//          | Nil -> 0
+//          | Cons (x, xsref) -> 
+//            let xs = !xsref in
+//             eliminate forall (a:Type) (c:witnessable a) (r:ref a). satisfy r h0 is_low_pred ==>
+//               c.satisfy (sel h0 r) h0 is_low_pred with (linkedList a) (solve) xsref;
+//             eliminate forall (a:Type) (c:witnessable a) (r:ref a). satisfy r h0 contains_pred ==>
+//               c.satisfy (sel h0 r) h0 contains_pred with (linkedList a) (solve) xsref;
+//             1 + length_IST a xs #c
+
+//  let rec length (a: Type0) (l: linkedList a) (h: lheap) {| c:target_lang a |} : nat 
+//        // (requires (fun h -> shallowly_contained l h /\ shallowly_low l h))
+//        =
+//        // let h0 = get() in
+//         match l with 
+//          | Nil -> 0
+//          | Cons (x, xsref) -> 
+//            let xs = sel h xsref in
+//             // eliminate forall (a:Type) (c:target_lang a) (r:ref a). shallowly_low r h0 ==>
+//             //   c.shallowly_low (sel h0 r) h0 with (linkedList a) (solve) xsref;
+//             // eliminate forall (a:Type) (c:target_lang a) (r:ref a). shallowly_contained r h0 ==>
+//             //   c.shallowly_contained (sel h0 r) h0 with (linkedList a) (solve) xsref;
+//             1 + length a xs h #c 
+
+let rec deep_high_ll (#a: Type0) (fuel: nat) (l: linkedList a) (h: lheap): Type0 =
+  if fuel = 0 then False
+  else
+    match l with
+    | Nil -> True
+    | Cons (x, xsref) -> 
+      label_of xsref h == High /\ deep_high_ll (fuel - 1) (sel h xsref) h
+
+noeq type deep_high_ll_ind (#a: Type0) (h: lheap) : linkedList a -> Type0 =
+| DH_Nil: deep_high_ll_ind #a h Nil
+| DH_Cons: x:a -> xsref: ref(linkedList a){label_of xsref h == High} ->
+    deep_high_ll_ind h (sel h xsref) ->
+    deep_high_ll_ind h (Cons (x, xsref))
+
+noeq type ll_constant_ind (#a: Type0) (h1 h2: lheap) : linkedList a -> Type0 =
 | LLC_Nil : ll_constant_ind h1 h2 (Nil #a)
 | LLC_Cons_Cons_Cons : v:a ->
     xsref:ref (linkedList a){sel h1 xsref == sel h2 xsref} ->
@@ -121,7 +144,7 @@ type ll_constant_ind (#a: Type0) (h1 h2: lheap) : linkedList a -> Type0 =
     ll_constant_ind h1 h2 (Cons (v,xsref))
 
 let rec ll_constant (#a: Type0) (fuel: nat) (l: linkedList a) (h1 h2: lheap) : Type0 =
-  if fuel = 0 then True
+  if fuel = 0 then False
   else
     match l with
     | Nil -> True
@@ -136,7 +159,41 @@ let rec ll_constant (#a: Type0) (fuel: nat) (l: linkedList a) (h1 h2: lheap) : T
         x == y /\ xsref == ysref /\ ll_constant (fuel - 1) xs1 h1 h2
     end
 
-// examples
+
+let rec footprint_acc
+  (#a: Type)
+  (l: linkedList a) 
+  (h:lheap) 
+  (hdom:(erased (FSet.set pos)){forall (a:Type) (rel:_) (r:mref a rel). h `contains` r ==> addr_of r `FSet.mem` hdom})
+  (acc:(erased (FSet.set pos)){acc `FSet.subset` hdom}) : 
+  Tot (erased (FSet.set pos)) (decreases (FSet.cardinality (hdom `FSet.difference` acc))) =
+  match l with 
+  | Nil -> acc
+  | Cons (x, xsref) -> 
+    if addr_of xsref `FSet.mem` acc then acc
+    else begin
+      assume (h `contains` xsref);
+      let acc' = (acc `FSet.union` FSet.singleton (addr_of xsref)) in
+      FSet.all_finite_set_facts_lemma ();
+      assert (acc' `FSet.subset` hdom);
+      assert ((hdom `FSet.difference` acc') `FSet.subset`
+              (hdom `FSet.difference` acc));
+      assert (~((hdom `FSet.difference` acc') `FSet.equal`
+              (hdom `FSet.difference` acc))); 
+      assert (FSet.cardinality (hdom `FSet.difference` acc') < 
+              FSet.cardinality (hdom `FSet.difference` acc));
+      footprint_acc (sel h xsref) h hdom acc' 
+    end
+
+let footprint (#a: Type) (l: linkedList a) (h:lheap) =
+  let hdom = get_hdom h in
+  assume (FSet.emptyset `FSet.subset` hdom);
+  footprint_acc l h hdom FSet.emptyset
+
+let separated (#a: Type) (l1 l2: linkedList a) (h: lheap): Type0 = 
+  (footprint l1 h `FSet.intersection` footprint l2 h) == FSet.emptyset
+
+(* Examples of linked lists *)
 
 let empty_ll: linkedList nat = Nil
 
@@ -160,155 +217,230 @@ let cycle_length3 () : ST (linkedList nat) (requires fun _ -> True) (ensures fun
 
 
 // TODO: clean up
-let rec deep_declassify (l: linkedList int) : ST unit 
-  (requires fun h -> shallowly_contained l h /\ inv_contains_points_to_contains h)
-  (ensures fun h0 x h1 ->
-    inv_contains_points_to_contains h1 /\
-    modifies Set.empty h0 h1 /\
-    shallowly_low l h1 /\
-    (forall (a:Type) (c:target_lang a) (r:ref a). 
-    (shallowly_contained r h0 /\ ~(shallowly_low r h0) /\ shallowly_low r h1) ==> c.shallowly_low (sel h1 r) h1)
-    ) =
-  let h0 = get() in
-  match l with 
-  | Nil -> ()
-  | Cons (h, tlref) ->
-      let tl = !tlref in 
-      declassify_low' tlref;
-      // gst_witness (is_low_pred tlref);
-      eliminate forall (a:Type) (c:target_lang a) (r:ref a). shallowly_contained r h0 ==>
-        c.shallowly_contained (sel h0 r) h0 with (linkedList int) (solve) tlref;
-      let h1 = get () in
-      // admit();
-      deep_declassify tl;
-      // admit();
-      let h2 = get () in
-      // assert ((forall (a:Type) (c:target_lang a) (r:ref a). h0 `contains` r <==> h1 `contains` r));
-      // assert ((forall (a:Type) (c:target_lang a) (r:ref a). 
-      //           (h1 `contains` r /\ label_of r h1 <> Low /\ label_of r h2 == Low) ==> 
-      //             c.shallowly_low (sel h2 r) h2));
+// let rec deep_declassify (l: linkedList int) : ST unit 
+//   (requires fun h -> satisfy l h contains_pred /\ inv_contains_points_to_contains h)
+//   (ensures fun h0 x h1 ->
+//     inv_contains_points_to_contains h1 /\
+//     modifies Set.empty h0 h1 /\
+//     (* TODO: modifies_classification (footprint l) h0 h1 *)
+//     satisfy l h1 is_low_pred /\
+//     (forall (a:Type) (c:witnessable a) (r:ref a). 
+//     (~(satisfy r h0 is_low_pred) /\ satisfy r h1 is_low_pred) ==> c.satisfy (sel h1 r) h1 is_low_pred)
+//     ) =
+//   let h0 = get() in
+//   match l with 
+//   | Nil -> ()
+//   | Cons (h, tlref) ->
+//       let tl = !tlref in 
+//       declassify_low' tlref;
+//       eliminate forall (a:Type) (c:witnessable a) (r:ref a). satisfy r h0 contains_pred ==>
+//         c.satisfy (sel h0 r) h0 contains_pred with (linkedList int) (solve) tlref;
+//       let h1 = get () in
+//       deep_declassify tl;
+//       let h2 = get () in
+//       introduce forall (a:Type) (c:witnessable a) (r:ref a). 
+//                (~(satisfy r h0 is_low_pred) /\ satisfy r h2 is_low_pred) ==> 
+//                 c.satisfy (sel h2 r) h2 is_low_pred
+//       with begin
+//         introduce (~(satisfy r h0 is_low_pred) /\ satisfy r h2 is_low_pred) ==> 
+//                 c.satisfy (sel h2 r) h2 is_low_pred
+//         with _. begin
+//           introduce ~(satisfy r h1 is_low_pred) ==> c.satisfy (sel h2 r) h2 is_low_pred with _. ();
+//           introduce satisfy r h1 is_low_pred ==> c.satisfy (sel h2 r) h2 is_low_pred with _. begin
+//             assert (addr_of r = addr_of tlref);
+//             assume (is_mm r = is_mm tlref);
+//             lemma_sel_same_addr' h2 r tlref;
+//             // assert (shallowly_low (sel h2 tlref) h2);
+//             // assert (sel h2 tlref == sel h2 r);
+//             let c : witnessable (linkedList int) = c in
+//             assert ((target_lang_linkedList int).satisfy (sel h2 tlref) h2 is_low_pred);
+//             assume ((forall (a:Type) (c:witnessable a) (c':witnessable a) (v:a) . 
+//               c.satisfy v h2 is_low_pred ==> c'.satisfy v h2 is_low_pred));
+//             assert (c.satisfy (sel h2 tlref) h2 is_low_pred);
+//             ()
+//           end
+//         end 
+//       end;
+//       ()
 
+// (* Tests *)
 
-      // assert (modifies_classification (only tlref) h0 h1);
-      // assert (modifies Set.empty h0 h2);
-      // assert (sel h0 tlref == sel h2 tlref);
-      // assert (shallowly_low (sel h2 tlref) h2);
-      // assert ((label_of tlref h0 <> Low /\ label_of tlref h2 == Low) ==> 
-      //           shallowly_low (sel h2 tlref) h2);   
-    
-      introduce forall (a:Type) (c:target_lang a) (r:ref a). 
-               (shallowly_contained r h0 /\ ~(shallowly_low r h0) /\ shallowly_low r h2) ==> 
-                c.shallowly_low (sel h2 r) h2
-      with begin
-        introduce (shallowly_contained r h0 /\ ~(shallowly_low r h0) /\ shallowly_low r h2) ==> 
-                c.shallowly_low (sel h2 r) h2
-        with _. begin
-          introduce ~(shallowly_low r h1) ==> c.shallowly_low (sel h2 r) h2 with _. ();
-          introduce shallowly_low r h1 ==> c.shallowly_low (sel h2 r) h2 with _. begin
-            assert (addr_of r = addr_of tlref);
-            lemma_sel_same_addr' h2 r tlref;
-            assert (shallowly_low (sel h2 tlref) h2);
-            assert (sel h2 tlref == sel h2 r);
-            // let r : ref (linkedList int) = r in
-            let c : target_lang (linkedList int) = c in
-            assert ((target_lang_linkedList int).shallowly_low (sel h2 tlref) h2);
-            assume ((forall (a:Type) (c:target_lang a) (c':target_lang a) (v:a) . 
-              c.shallowly_low v h2 ==> c'.shallowly_low v h2));
-            assert (c.shallowly_low (sel h2 tlref) h2);
-            assert (c.shallowly_low (sel h2 r) h2);
-            ()
-          end
-        end 
-      end;
-      ()
+// // TODO: Review this
+// let test_declassify (l: linkedList int) : IST unit 
+//   (ensures fun h -> shallowly_contained l h) 
+//   (requires fun _ _ _ -> True) =
+//   let h0 = get() in
+//   deep_declassify l;
+//   let h1 = get() in
+//   // assume ((forall (a:Type) (c:target_lang a) (c':target_lang a) (v:a) . 
+//   //   (target_lang_ref a #c).shallowly_low v h1 ==> c'.shallowly_low v h1));
 
-  // Tests
+//   assert (modifies Set.empty h0 h1);
+//   assert (shallowly_contained l h0);
+//   assert (shallowly_contained l h1);
+//   assert (inv_contains_points_to_contains h1);
 
+//   assert (shallowly_low l h1);
+//   assert (inv_low_points_to_low h0); // by IST
 
-// review this later
-let test_declassify (l: linkedList int) : IST unit (ensures fun h -> shallowly_contained l h) (requires fun _ _ _ -> True) =
-  // deep_declassify l;
-  // let h2 = get() in
-  // assume ((forall (a:Type) (c:target_lang a) (c':target_lang a) (v:a) . 
-  //            c.shallowly_low v h2 ==> c'.shallowly_low v h2));
-  ()
+//   introduce forall (a:Type) (c:target_lang a) (r:ref a).
+//     shallowly_low r h1 ==> c.shallowly_low (sel h1 r) h1
+//   with begin
+//     introduce shallowly_low r h1 ==> c.shallowly_low (sel h1 r) h1 with _. begin
+//       introduce shallowly_low r h0 ==> c.shallowly_low (sel h1 r) h1 with _. begin
+//         assert (h0 `contains` r);
+//         assert (modifies_none h0 h1);
+//         assert (sel h1 r == sel h0 r);
+//         assert (shallowly_low r h0 ==> c.shallowly_low (sel h0 r) h0);
+//         lemma (sel h1 r) h0 h1;
+//         // assume (shallowly_low (sel h1 r) h0 ==> shallowly_low (sel h1 r) h1);
+//         ()
+//       end;
+//       introduce ~(shallowly_low r h0) ==> c.shallowly_low (sel h1 r) h1 with _. begin
+//         assert
+//           ((~(shallowly_low r h0) /\ shallowly_low r h1) ==> c.shallowly_low (sel h1 r) h1);
+//         assert (~(shallowly_low r h0));
+//         assert (shallowly_low r h1);
+//         ()
+//       end
+//     end
+//   end;
 
-val progr_linked_list_unchanged: 
-  rp: ref (linkedList int) -> 
-  rs: ref int ->
-  ctx:(elab_typ (TArr TUnit TUnit)) ->
-  IST unit 
-    (requires (fun h0 -> 
-      shallowly_contained rp h0 /\
-      label_of rp h0 == High /\
-      shallowly_low rs h0))
-    (ensures (fun h0 _ h1 ->
-      sel h0 rp == sel h1 rp))
-         
-let progr_secret_unchanged_test rp rs ctx = 
-  let x = alloc Nil in 
-  let y = alloc (Cons (31, x)) in
-  let secret_ll = Cons(23, y) in
-  ctx ();
-  // assert (head int secret_ll == 31); // how to cast type?
-  // assert (head int (tail int secret_ll) == 23);
-  ()
-
-// val ctx_HO :
-//   elab_typ (TArr (TArr TUnit (TRef TNat)) TUnit)
-// let ctx_HO f =
-//   let h0 = get () in
-//   let x:ref int = f () in
-//   let y = alloc Nil in
-//   let z = Cons(!x, y) in
-//   let t = insert_front int z 13 in
-//   let h2 = get () in
-//   assert (modifies_only_label Low h0 h2);
+//   assert (inv_low_points_to_low h1);
 //   ()
 
-// test with program getting callback?
+// let test2_declassify (l1 l2: linkedList int) : IST unit 
+//   (ensures fun h -> shallowly_contained l1 h /\ shallowly_contained l2 h /\ deep_high_ll l2 h) 
+//   (requires fun _ _ h1 -> deep_high_ll l2 h1) =
+//   deep_declassify l1;
 
 
-// how to check all labels of a list are High (esp. for cycles?)?
-// val progr_sep:
+// // val progr_linked_list_unchanged: 
+// //   rp: ref (linkedList int) -> 
+// //   rs: ref int ->
+// //   ctx:(elab_typ (TArr TUnit TUnit)) ->
+// //   IST unit 
+// //     (requires (fun h0 -> 
+// //       shallowly_contained rp h0 /\
+// //       label_of rp h0 == High /\
+// //       shallowly_low rs h0))
+// //     (ensures (fun h0 _ h1 ->
+// //       sel h0 rp == sel h1 rp))
+         
+// // let progr_secret_unchanged_test rp rs ctx = 
+// //   let x = alloc Nil in 
+// //   let y = alloc (Cons (31, x)) in
+// //   let secret_ll = Cons(23, y) in
+// //   ctx ();
+// //   let h = get() in
+// //   assert (head int secret_ll h == 31);
+// //   // assert (head int (tail int secret_ll) == 23);
+// //   ()
+
+// // val ctx_HO :
+// //   elab_typ (TArr (TArr TUnit (TRef TNat)) TUnit)
+// // let ctx_HO f =
+// //   let h0 = get () in
+// //   let x:ref int = f () in
+// //   let y = alloc Nil in
+// //   let z = Cons(!x, y) in
+// //   let t = insert_front int z 13 in
+// //   let h2 = get () in
+// //   assert (modifies_only_label Low h0 h2);
+// //   ()
+
+// // test with program getting callback?
+
+// // val progr_sep:
+// //   rp: linkedList int -> 
+// //   ctx:(elab_typ (TArr (TRef TNat) TUnit)) ->
+// //   IST unit
+// //     (requires (fun h0 -> 
+// //       shallowly_contained rp h0 /\
+// //       label_of (last rp) h0 == High)
+// //     )
+// //     (ensures (fun h0 _ h1 -> True))
+// // let progr_sep rp f =
+// //   deep_declassify rp;
+// //   let h1 = get () in
+// //   assume (inv_low_points_to_low h1);
+// //   let r = f rp in  
+// //   r
+
+// // add precond of not cycles
+// let rec lemma_list_unchanged_modif_none (#a: Type0) (rp: linkedList a) (h0 h1: lheap): Lemma
+//   (requires modifies_none h0 h1)
+//   (ensures exists (gas:nat) . ll_constant gas rp h0 h1)
+//   (decreases rp) = 
+//   match rp with
+//   | Nil ->
+//     assert (ll_constant 1 rp h0 h1);
+//     ()
+//   | Cons (x, xsref) -> 
+//     let xs1 = sel h0 xsref in
+//     let xs2 = sel h1 xsref in
+//     assert (modifies Set.empty h0 h1);
+//     assume (h0 `contains` xsref);
+//     assert (xs1 == xs2);
+//     admit();
+//     lemma_list_unchanged_modif_none xs1 h0 h1;
+//     ()
+
+// let lemma_list_unchanged_when_high (#a: Type0) (rp: linkedList a) (h0 h1: lheap): Lemma
+//   (requires (exists (gas: nat). deep_high_ll gas rp h0 /\ modifies_only_label Low h0 h1))
+//   (ensures exists (gas: nat). ll_constant gas rp h0 h1)
+//   (decreases rp) = 
+//   match rp with
+//   | Nil ->
+//     assert (ll_constant 1 rp h0 h1);
+//     ()
+//   | Cons (x, xsref) -> 
+//     let xs1 = sel h0 xsref in
+//     let xs2 = sel h1 xsref in
+//     // assert (modifies Set.empty h0 h1);
+//     // assume (h0 `contains` xsref);
+//     // assert (xs1 == xs2);
+//     admit();
+//     // lemma_list_unchanged_modif_none xs1 h0 h1;
+//     ()
+
+// val progr_ll_unchanged':
 //   rp: linkedList int -> 
-//   ctx:(elab_typ (TArr (TRef TNat) TUnit)) ->
+//   ctx:(elab_typ (TArr TUnit TUnit)) ->
 //   IST unit
 //     (requires (fun h0 -> 
-//       shallowly_contained rp h0 /\
-//       // label_of (last rp) h0 == High)
+//       exists (gas: nat) . deep_high_ll gas rp h0 /\
+//       shallowly_contained rp h0
 //     ))
-//     (ensures (fun h0 _ h1 -> True))
-// let progr_sep rp f =
-//   deep_declassify rp;
-//   let h1 = get () in
-//   assume (inv_low_points_to_low h1);
-//   let r = f rp in  
-//   r
+//     (ensures (fun h0 _ h1 -> exists (gas: nat). ll_constant gas rp h0 h1))
+// let progr_ll_unchanged' rp f =
+//   let h0 = get () in
+//   f ();
+//   let h1 = get() in
+//   lemma_list_unchanged_when_high rp h0 h1;
+//   ()
 
-// val lemma_list_unchanged_when_high (#a: Type0) (rp: linkedList a) (h0 h1: lheap): Lemma {
+// // val ctx_alloc_ll: int -> St linked // take pre/post from elab_typ
+// // elab_typ (TArr TNat (TPair TNat (TRef TNat)))
+// // let ctx_alloc_ll v =
+// //   let r = alloc Nil in 
+// //   let rs = Cons(v, r) in
+// //   rs
 
-// }
-
-
-let rec deep_high_ll (#a: Type0) (fuel: nat) (l: linkedList a) (h: lheap): Type0 =
-  if fuel = 0 then True
-  else
-    match l with
-    | Nil -> True
-    | Cons (x, xsref) -> 
-      label_of xsref h == High /\ deep_high_ll (fuel - 1) (sel h xsref) h
-
-val progr_ll_unchanged':
-  rp: linkedList int -> 
-  ctx:(elab_typ (TArr TUnit TUnit)) ->
-  IST unit
-    (requires (fun h0 -> 
-      (forall gas . deep_high_ll gas rp h0) /\
-      shallowly_contained rp h0
-    ))
-    (ensures (fun h0 _ h1 ->  forall gas . ll_constant gas rp h0 h1))
-let progr_ll_unchanged' rp f =
-  let h1 = get () in
-  f ();
-  ()
+// // val progr_passes_cb:
+// //   rp: linkedList int ->
+// //   ctx: (elab_typ (TArr (TArr TUnit TUnit) TUnit)) ->
+// //   IST unit 
+// //     (requires fun h0 -> 
+// //       shallowly_contained rp h0 /\ 
+// //       (exists (gas: nat) . deep_high_ll gas rp h0))
+// //     (ensures fun _ _  h1 -> inv_low_points_to_low h1)
+// // let progr_getting_callback_test rp ctx = 
+// //   declassify_low' (last_ref rp); // this shouldn't be necessary (the cb of the program should be able to modify High things)
+// //   let cb: elab_typ (TArr TUnit TUnit) = 
+// //     (fun () -> 
+// //       let last_of_ll = last rp in
+// //       write' last_of_ll (!last_of_ll + 1)) in
+// //   ctx cb;
+// //   ()
+    
