state/TargetLangIFC.fst
@@ -10,6 +10,10 @@ open IFC.Heap.ST
 type ref_lheap_pred =
   pred:(#a:Type -> #rel:_ -> mref a rel -> lheap -> Type0){forall (a:Type) (x:ref a) h0 h1. pred x h0 /\ h0 `lheap_rel` h1 ==> pred x h1}
 
+noeq type linkedList (a: Type0) : Type0 =
+    | Nil
+    | Cons of a * ref (linkedList a)
+
 class witnessable (t:Type) = {
   satisfy : t -> lheap -> ref_lheap_pred -> Type0;
 
@@ -77,6 +81,30 @@ instance witnessable_sum (t1:Type) (t2:Type) {| c1:witnessable t1 |} {| c2:witne
     | Inr x2 -> (let w = c2.witness x2 pred in (fun () -> w ())))
 }
 
+instance witnessable_llist (t:Type) {| c:witnessable t |} : witnessable (linkedList t) = {
+  satisfy = (fun l h pred -> 
+    match l with
+    | Nil -> True
+    | Cons (x, xsref) -> c.satisfy x h pred /\ pred xsref h
+  );
+
+  satisfy_monotonic = (fun l pred h0 h1 ->
+    match l with 
+    | Nil -> ()
+    | Cons (x, xsref) -> c.satisfy_monotonic x pred h0 h1
+  );
+
+  witness = (fun l pred ->
+    match l with
+    | Nil -> (fun () -> ())
+    | Cons (x, xsref) ->
+      let w = c.witness x pred in
+      mst_witness (pred xsref);
+      (fun () -> w ();
+      mst_recall (pred xsref))
+  );
+}
+
 (** *** Elaboration of types to F* *)
 
 unfold let shallowly_contained_low (#a:Type) {| c:witnessable a |} (v:a) (h:lheap) =
@@ -131,9 +159,9 @@ let rec _elab_typ (t:typ) (inv:lheap -> Type0): tt:Type0 & witnessable tt =
   | TRef t ->
     let (| tt, c_tt |) = _elab_typ t inv in
     (| ref tt, witnessable_ref tt #c_tt |)
-  | TLList t -> admit ()
-    // let (| tt, c_tt |) = _elab_typ t inv in
-    // (| list tt, witnessable_llist tt #c_tt |)
+  | TLList t ->
+    let (| tt, c_tt |) = _elab_typ t inv in
+    (| linkedList tt, witnessable_llist tt #c_tt |)
 
 let inv_contains_points_to_contains (h:lheap) =
   (forall (a:typ) (inv:lheap -> Type0).
